proof/Demorgan.lean
@@ -1,4 +1,0 @@
-import Demorgan.Basic
-import Demorgan.ListMax
-import Demorgan.ReverseInvolution
-import Demorgan.Trie
